feat(init/category/transformers): add `monad_run` class

tests/lean/run/isabelle.lean
@@ -71,7 +71,7 @@ meta instance : alternative lazy_tactic :=
 meta def choose {α} (xs : list α) : lazy_tactic α :=
 λ s, of_list $ xs^.map (λ a, (a, s))
 
-meta def run {α} (t : lazy_tactic α) : tactic α :=
+protected meta def run {α} (t : lazy_tactic α) : tactic α :=
 λ s, match t s with
 | nil                := tactic.failed s
 | cons (a, new_s) ss := result.success a new_s
@@ -94,7 +94,7 @@ end lazy_tactic
 open lazy_tactic
 
 example (p q : Prop) : q → p ∨ q :=
-by run $ do
+by lazy_tactic.run $ do
  tactic.intros,
  constructor,
  tactic.trace_state,
